ulib/Steel.Pointer.fsti
@@ -1,0 +1,105 @@
+(*
+   Copyright 2008-2019 Microsoft Research
+
+   Licensed under the Apache License, Version 2.0 (the "License");
+   you may not use this file except in compliance with the License.
+   You may obtain a copy of the License at
+
+       http://www.apache.org/licenses/LICENSE-2.0
+
+   Unless required by applicable law or agreed to in writing, software
+   distributed under the License is distributed on an "AS IS" BASIS,
+   WITHOUT WARRANTIES OR CONDITIONS OF ANY KIND, either express or implied.
+   See the License for the specific language governing permissions and
+   limitations under the License.
+*)
+module Steel.Pointer
+
+module P = LowStar.Permissions
+module A = LowStar.Array
+
+include Steel.Pointer.Views
+
+open Steel.RST
+
+(**** Unscoped allocation and deallocation of pointer resources *)
+
+val ptr_alloc
+  (#a:Type)
+  (init:a)
+  : RST (pointer a)
+    (empty_resource)
+    (fun ptr -> ptr_resource ptr)
+    (fun _ -> True)
+    (fun _ ptr h1 ->
+      A.freeable ptr /\
+      get_val ptr h1 == init /\
+      get_perm ptr h1 = FStar.Real.one
+    )
+
+val ptr_free
+  (#a:Type)
+  (ptr:pointer a)
+  : RST unit
+    (ptr_resource ptr)
+    (fun ptr -> empty_resource)
+    (fun h0 -> A.freeable ptr /\ P.allows_write (get_perm ptr h0))
+    (fun _ _ _ -> True)
+
+(**** Reading and writing using a pointer resource *)
+
+val ptr_read
+  (#a:Type)
+  (ptr:pointer a)
+  : RST a
+    (ptr_resource ptr)
+    (fun _ -> ptr_resource ptr)
+    (fun _ -> True)
+    (fun h0 x h1 ->
+      get_val ptr h0 == x /\
+      h0 == h1
+    )
+
+val ptr_write
+  (#a:Type)
+  (ptr:pointer a)
+  (x:a)
+  : RST unit
+    (ptr_resource ptr)
+    (fun _ -> ptr_resource ptr)
+    (fun h0 -> P.allows_write (get_perm ptr h0))
+    (fun h0 _ h1 ->
+      get_perm ptr h0 == get_perm ptr h1 /\
+      get_val ptr h1 == x
+    )
+
+val ptr_share
+  (#a: Type)
+  (ptr: pointer a)
+  : RST (pointer a)
+    (ptr_resource ptr)
+    (fun ptr1 -> ptr_resource ptr <*> ptr_resource ptr1)
+    (fun _ -> True)
+    (fun h0 ptr1 h1 ->
+      get_val ptr h1 == get_val ptr h0  /\
+      get_val ptr1 h1 == get_val ptr h0  /\
+      get_perm ptr h1 == P.half_permission (get_perm ptr h0) /\
+      get_perm ptr1 h1 == P.half_permission (get_perm ptr h0) /\
+      A.gatherable ptr ptr1 /\
+      P.summable_permissions (get_perm ptr h1) (get_perm ptr1 h1))
+
+val ptr_merge
+  (#a: Type)
+  (ptr1: pointer a)
+  (ptr2: pointer a)
+  : RST unit
+    (ptr_resource ptr1 <*> ptr_resource ptr2)
+    (fun _ -> ptr_resource ptr1)
+    (fun h0 -> A.gatherable ptr1 ptr2 /\
+      P.summable_permissions (get_perm ptr1 h0) (get_perm ptr2 h0)
+    )
+    (fun h0 _ h1 ->
+      P.summable_permissions (get_perm ptr1 h0) (get_perm ptr2 h0) /\
+      get_val ptr1 h1 == get_val ptr1 h0 /\
+      get_perm ptr1 h1 == P.sum_permissions (get_perm ptr1 h0) (get_perm ptr2 h0)
+     )
